Use the standard direction of <= for abs interp

src/Parsers/ContextFreeGrammar/Fix/Definitions.v
@@ -8,46 +8,150 @@ Require Import Fiat.Common.Notations.
 Set Implicit Arguments.
 
 Local Coercion is_true : bool >-> Sortclass.
+Delimit Scope grammar_fixedpoint_scope with fixedpoint.
+Local Open Scope grammar_fixedpoint_scope.
 
-Class grammar_fixedpoint_lattice_data state :=
-  { state_lt : state -> state -> bool;
-    state_beq : state -> state -> bool;
+Inductive lattice_for T := top | constant (_ : T) | bottom.
+Bind Scope grammar_fixedpoint_scope with lattice_for.
+Scheme Equality for lattice_for.
+
+Arguments bottom {_}.
+Arguments top {_}.
+Notation "'⊥'" := bottom : grammar_fixedpoint_scope.
+Notation "'⊤'" := top : grammar_fixedpoint_scope.
+
+Definition lattice_for_lt {T} (lt : T -> T -> bool) (x y : lattice_for T)
+  := match x, y with
+     | ⊤, ⊤ => false
+     | constant x', constant y' => lt x' y'
+     | ⊥, ⊥ => false
+     | _, ⊤ => true
+     | ⊤, _ => false
+     | _, constant _ => true
+     | constant _, _ => false
+     end.
+
+Definition lattice_for_lub {T} (lub : T -> T -> lattice_for T) (x y : lattice_for T)
+  := match x, y with
+     | ⊤, ⊤ => ⊤
+     | constant x', constant y' => lub x' y'
+     | ⊥, ⊥ => ⊥
+     | ⊤, _
+     | _, ⊤
+       => ⊤
+     | ⊥, v
+     | v, ⊥
+       => v
+     end.
+
+Section lub_correct.
+  Context {T} (beq : T -> T -> bool) (lt : T -> T -> bool) (lub : T -> T -> lattice_for T).
+
+  Local Notation "x <= y" := (orb (lattice_for_beq beq x y) (lattice_for_lt lt x y)).
+
+  Context (lub_correct_l : forall x y, constant x <= lub x y)
+          (lub_correct_r : forall x y, constant y <= lub x y)
+          (beq_refl : forall x y, x = y -> beq x y).
+
+  Lemma lattice_for_lub_correct_l x y
+    : x <= lattice_for_lub lub x y.
+  Proof.
+    clear lub_correct_r.
+    destruct x as [|x|], y as [|y|]; try reflexivity.
+    { exact (lub_correct_l x y). }
+    { simpl.
+      rewrite beq_refl by reflexivity; reflexivity. }
+  Qed.
+
+  Lemma lattice_for_lub_correct_r x y
+    : y <= lattice_for_lub lub x y.
+  Proof.
+    clear lub_correct_l.
+    destruct x as [|x|], y as [|y|]; try reflexivity.
+    { exact (lub_correct_r x y). }
+    { simpl.
+      rewrite beq_refl by reflexivity; reflexivity. }
+  Qed.
+End lub_correct.
+
+Definition lattice_for_gt_well_founded {T} {lt : T -> T -> bool}
+           (gt_wf : well_founded (Basics.flip lt))
+  : well_founded (Basics.flip (lattice_for_lt lt)).
+Proof.
+  do 3 (constructor;
+        repeat match goal with
+               | [ v : T, H : well_founded _ |- _ ] => specialize (H v); induction H
+               | [ x : lattice_for _ |- _ ] => destruct x
+               | _ => progress simpl in *
+               | _ => progress unfold Basics.flip in *
+               | [ H : is_true false |- _ ] => exfalso; clear -H; abstract congruence
+               | _ => intro
+               | _ => solve [ eauto with nocore ]
+               end).
+Defined.
+
+Global Instance lattice_for_lt_Transitive {T} {lt : T -> T -> bool} {_ : Transitive lt}
+  : Transitive (lattice_for_lt lt).
+Proof.
+  intros [|?|] [|?|] [|?|]; simpl; trivial; try congruence; [].
+  intros.
+  etransitivity; eassumption.
+Qed.
+
+Class grammar_fixedpoint_lattice_data prestate :=
+  { state :> _ := lattice_for prestate;
+    prestate_lt : prestate -> prestate -> bool;
+    state_lt : state -> state -> bool
+    := lattice_for_lt prestate_lt;
+    prestate_beq : prestate -> prestate -> bool;
+    state_beq : state -> state -> bool
+    := lattice_for_beq prestate_beq;
+    prestate_le s1 s2 := (prestate_beq s1 s2 || prestate_lt s1 s2)%bool;
     state_le s1 s2 := (state_beq s1 s2 || state_lt s1 s2)%bool;
-    state_beq_refl : forall s, state_beq s s;
-    state_beq_bl : forall s1 s2, state_beq s1 s2 -> s1 = s2;
-    greatest_lower_bound : state -> state -> state;
-    greatest_lower_bound_correct_l
-    : forall a b, state_le (greatest_lower_bound a b) a;
-    greatest_lower_bound_correct_r
-    : forall a b, state_le (greatest_lower_bound a b) b;
-    (*greatest_lower_bound_greatest
-    : forall a b c, state_le c a -> state_le c b -> state_le c (greatest_lower_bound a b);*)
-    initial_state : state;
-    bottom : state;
-    bottom_bottom : forall st, state_le bottom st;
-    state_lt_wf : well_founded state_lt;
-    state_lt_Transitive : Transitive state_lt }.
+    prestate_beq_lb : forall s1 s2, s1 = s2 -> prestate_beq s1 s2;
+    prestate_beq_bl : forall s1 s2, prestate_beq s1 s2 -> s1 = s2;
+    state_beq_lb : forall s1 s2, s1 = s2 -> state_beq s1 s2
+    := internal_lattice_for_dec_lb _ prestate_beq_lb;
+    state_beq_bl : forall s1 s2, state_beq s1 s2 -> s1 = s2
+    := internal_lattice_for_dec_bl _ prestate_beq_bl;
+    preleast_upper_bound : prestate -> prestate -> state;
+    least_upper_bound : state -> state -> state
+    := lattice_for_lub preleast_upper_bound;
+    preleast_upper_bound_correct_l
+    : forall a b, state_le (constant a) (preleast_upper_bound a b);
+    preleast_upper_bound_correct_r
+    : forall a b, state_le (constant b) (preleast_upper_bound a b);
+    least_upper_bound_correct_l
+    : forall a b, state_le a (least_upper_bound a b)
+    := lattice_for_lub_correct_l prestate_beq prestate_lt preleast_upper_bound preleast_upper_bound_correct_l prestate_beq_lb;
+    least_upper_bound_correct_r
+    : forall a b, state_le b (least_upper_bound a b)
+    := lattice_for_lub_correct_r prestate_beq prestate_lt preleast_upper_bound preleast_upper_bound_correct_r prestate_beq_lb;
+    prestate_gt_wf : well_founded (Basics.flip prestate_lt);
+    state_gt_wf : well_founded (Basics.flip state_lt)
+    := lattice_for_gt_well_founded prestate_gt_wf;
+    prestate_lt_Transitive : Transitive prestate_lt;
+    state_lt_Transitive : Transitive state_lt
+    := lattice_for_lt_Transitive }.
 
 Record grammar_fixedpoint_data :=
-  { state :> Type;
-    lattice_data :> grammar_fixedpoint_lattice_data state;
+  { prestate : Type;
+    lattice_data :> grammar_fixedpoint_lattice_data prestate;
     step_constraints : (default_nonterminal_carrierT -> state) -> (default_nonterminal_carrierT -> state -> state);
     step_constraints_ext : Proper (pointwise_relation _ eq ==> eq ==> eq ==> eq) step_constraints }.
 
 Global Existing Instance lattice_data.
 Global Existing Instance step_constraints_ext.
+Global Existing Instance state_lt_Transitive.
 
-Delimit Scope grammar_fixedpoint_scope with fixedpoint.
-Local Open Scope grammar_fixedpoint_scope.
+Global Arguments state_lt_Transitive {_ _} [_ _ _] _ _.
+Global Arguments state_le _ _ !_ !_ / .
+Global Arguments state {_ _}, {_} _.
 
 Infix "<=" := (@state_le _ _) : grammar_fixedpoint_scope.
 Infix "<" := (@state_lt _ _) : grammar_fixedpoint_scope.
-Infix "⊓" := (@greatest_lower_bound _ _) : grammar_fixedpoint_scope.
+Infix "⊔" := (@least_upper_bound _ _) : grammar_fixedpoint_scope.
 Infix "=b" := (@state_beq _ _) : grammar_fixedpoint_scope.
-Notation "'⊥'" := (@bottom _ _) : grammar_fixedpoint_scope.
-
-Arguments state_lt_Transitive {_ _} [_ _ _] _ _.
-Global Existing Instance state_lt_Transitive.
 
 Definition nonterminal_to_positive (nt : default_nonterminal_carrierT) : positive
   := Pos.of_nat (S nt).
