src/Parsers/ContextFreeGrammar/Fix/Correct.v
@@ -22,12 +22,12 @@ Section grammar_fixedpoint.
   Lemma pre_Fix_grammar_fixedpoint_correct_valid
         (P : default_nonterminal_carrierT -> state gdata -> Type)
         (Pinit : forall nt, is_true (is_valid_nonterminal initial_nonterminals_data nt)
-                            -> P nt (initial_state (*nt*)))
+                            -> P nt ⊥)
         (IH : forall nt st v,
             st nt = v
             -> is_true (is_valid_nonterminal initial_nonterminals_data nt)
             -> P nt v
-            -> P nt (v ⊓ step_constraints gdata st nt v))
+            -> P nt (v ⊔ step_constraints gdata st nt v))
     : forall nt, is_true (is_valid_nonterminal initial_nonterminals_data nt) -> P nt (lookup_state (pre_Fix_grammar gdata initial_nonterminals_data) nt).
   Proof.
     specialize (fun nt st => IH nt st _ eq_refl).
@@ -49,7 +49,7 @@ Section grammar_fixedpoint.
       eauto. }
     pose proof (fun nt (pf : is_true (is_valid_nonterminal (@initial_nonterminals_data _ (@rdp_list_predata _ G)) nt))
                 => match eq_sym pf in (_ = b)
-                         return (if b then initial_state (*nt*) else ⊥) =
+                         return (if b then ⊥ else ⊤) =
                                 lookup_state (aggregate_state_max gdata initial_nonterminals_data) nt
                                 -> _
                    with
@@ -64,14 +64,8 @@ Section grammar_fixedpoint.
     rewrite Init.Wf.Fix_eq by (intros; edestruct Sumbool.sumbool_of_bool; trivial).
     edestruct Sumbool.sumbool_of_bool; [ intros; apply Pinit'; assumption | ].
     fold (pre_Fix_grammar_helper (gdata := gdata) initial_nonterminals_data) in *.
-    destruct (aggregate_state_eq (aggregate_step a) a) eqn:Heq.
-    { change (is_true (aggregate_state_eq (aggregate_step a) a)) in Heq.
-      intros nt Hvalid.
-      remember (lookup_state (pre_Fix_grammar_helper (@initial_nonterminals_data _ predata) (aggregate_step a)) nt) as st eqn:Hst.
-      rewrite pre_Fix_grammar_helper_fixed in Hst by (rewrite !Heq; reflexivity).
-      rewrite Heq in Hst.
-      subst.
-      eauto. }
+    destruct (aggregate_state_eq a (aggregate_step a)) eqn:Heq.
+    { intuition congruence. }
     { apply step_lt in Heq.
       intros nt.
       apply IHa; eauto; intros; try apply IH;
@@ -85,7 +79,7 @@ Section grammar_fixedpoint.
                | _ => progress unfold lookup_state, option_map, option_rect in *
                | [ H : forall nt, is_true (?P nt) -> _, H' : is_true (?P _) |- _ ]
                  => specialize (H _ H')
-               | [ |- ?P ?nt (_ ⊓ _) ] => apply P_glb
+               | [ |- ?P ?nt (_ ⊔ _) ] => apply P_lub
                | [ H : context[match ?e with _ => _ end] |- _ ] => destruct e eqn:?
                | [ |- context[match ?e with _ => _ end] ] => destruct e eqn:?
                end. }
@@ -93,15 +87,15 @@ Section grammar_fixedpoint.
 
   Lemma pre_Fix_grammar_fixedpoint_correct
         (P : default_nonterminal_carrierT -> state gdata -> Type)
-        (Pinit : forall nt, is_true (is_valid_nonterminal initial_nonterminals_data nt)
-                            -> P nt (initial_state (*nt*)))
-        (Pbot : forall nt, is_valid_nonterminal initial_nonterminals_data nt = false
-                           -> P nt ⊥)
+        (Pbot : forall nt, is_true (is_valid_nonterminal initial_nonterminals_data nt)
+                          -> P nt ⊥)
+        (Ptop : forall nt, is_valid_nonterminal initial_nonterminals_data nt = false
+                           -> P nt ⊤)
         (IH : forall nt st v,
             st nt = v
             -> is_true (is_valid_nonterminal initial_nonterminals_data nt)
             -> P nt v
-            -> P nt (v ⊓ step_constraints gdata st nt v))
+            -> P nt (v ⊔ step_constraints gdata st nt v))
     : forall nt, P nt (lookup_state (pre_Fix_grammar gdata initial_nonterminals_data) nt).
   Proof.
     intro nt.
@@ -112,17 +106,17 @@ Section grammar_fixedpoint.
 
   Lemma pre_Fix_grammar_fixedpoint_correct_stronger'
         (P : default_nonterminal_carrierT -> state gdata -> Type)
-        (Pinit : forall nt, is_true (is_valid_nonterminal initial_nonterminals_data nt)
-                            -> P nt (initial_state (*nt*)))
-        (Pbot : forall nt, is_valid_nonterminal initial_nonterminals_data nt = false
-                           -> P nt ⊥)
+        (Pbot : forall nt, is_true (is_valid_nonterminal initial_nonterminals_data nt)
+                          -> P nt ⊥)
+        (Ptop : forall nt, is_valid_nonterminal initial_nonterminals_data nt = false
+                           -> P nt ⊤)
         (IH : forall nt st,
-            (forall nt', is_valid_nonterminal initial_nonterminals_data nt' = false -> st nt' = ⊥)
+            (forall nt', is_valid_nonterminal initial_nonterminals_data nt' = false -> st nt' = ⊤)
             -> (forall nt', P nt' (st nt'))
-            -> P nt (st nt ⊓ step_constraints gdata st nt (st nt)))
+            -> P nt (st nt ⊔ step_constraints gdata st nt (st nt)))
     : forall nt, is_true (is_valid_nonterminal initial_nonterminals_data nt) -> P nt (lookup_state (pre_Fix_grammar gdata initial_nonterminals_data) nt).
   Proof.
-    assert (Hbot : forall nt', is_valid_nonterminal initial_nonterminals_data nt' = false -> lookup_state (aggregate_state_max gdata initial_nonterminals_data) nt' = ⊥).
+    assert (Htop : forall nt', is_valid_nonterminal initial_nonterminals_data nt' = false -> lookup_state (aggregate_state_max gdata initial_nonterminals_data) nt' = ⊤).
     { intros nt' Hinvalid.
       simpl rewrite lookup_state_aggregate_state_max; simpl in *; rewrite Hinvalid.
       reflexivity. }
@@ -144,30 +138,24 @@ Section grammar_fixedpoint.
     pose proof (fun nt
                 => match is_valid_nonterminal (@initial_nonterminals_data _ (@rdp_list_predata _ G)) nt as b
                          return is_valid_nonterminal (@initial_nonterminals_data _ (@rdp_list_predata _ G)) nt = b
-                                -> (if b then initial_state (*nt*) else ⊥) =
+                                -> (if b then ⊥ else ⊤) =
                                    lookup_state (aggregate_state_max gdata initial_nonterminals_data) nt
                                 -> _
                    with
-                   | true => fun pf => eq_rect _ (P nt) (Pinit _ pf) _
-                   | false => fun pf => eq_rect _ (P nt) (Pbot _ pf) _
+                   | true => fun pf => eq_rect _ (P nt) (Pbot _ pf) _
+                   | false => fun pf => eq_rect _ (P nt) (Ptop _ pf) _
                    end eq_refl (eq_sym (lookup_state_aggregate_state_max gdata G nt))) as Pinit'.
     unfold pre_Fix_grammar, pre_Fix_grammar_helper.
     let Rwf := lazymatch goal with |- appcontext[Fix ?Rwf _ _ ?v] => Rwf end in
     let v := lazymatch goal with |- appcontext[Fix Rwf _ _ ?v] => v end in
     pose proof (fun nt => IH nt (lookup_state v)) as IHv;
-      specialize (fun nt => IHv nt Hbot Pinit');
+      specialize (fun nt => IHv nt Htop Pinit');
       induction (Rwf v) as [a Ha IHa].
     rewrite Init.Wf.Fix_eq by (intros; edestruct Sumbool.sumbool_of_bool; trivial).
     edestruct Sumbool.sumbool_of_bool; [ intros; apply Pinit'; assumption | ].
     fold (pre_Fix_grammar_helper (gdata := gdata) initial_nonterminals_data) in *.
-    destruct (aggregate_state_eq (aggregate_step a) a) eqn:Heq.
-    { change (is_true (aggregate_state_eq (aggregate_step a) a)) in Heq.
-      intros nt Hvalid.
-      remember (lookup_state (pre_Fix_grammar_helper (@initial_nonterminals_data _ predata) (aggregate_step a)) nt) as st eqn:Hst.
-      rewrite pre_Fix_grammar_helper_fixed in Hst by (rewrite !Heq; reflexivity).
-      rewrite Heq in Hst.
-      subst.
-      eauto. }
+    destruct (aggregate_state_eq a (aggregate_step a)) eqn:Heq.
+    { intuition congruence. }
     { apply step_lt in Heq.
       intros nt.
       simpl @nonterminal_carrierT in *.
@@ -186,8 +174,8 @@ Section grammar_fixedpoint.
                | [ H : is_true true -> _ |- _ ] => specialize (H eq_refl)
                | [ |- is_true true ] => reflexivity
                | [ |- is_true false ] => exfalso
-               | [ |- ?P ?nt (_ ⊓ _) ] => apply P_glb
-               | _ => rewrite bottom_glb_l
+               | [ |- ?P ?nt (_ ⊔ _) ] => apply P_lub
+               | _ => rewrite top_lub_l
                | [ H : Some _ = Some _ |- _ ] => inversion H; clear H
                | [ H : forall nt : default_nonterminal_carrierT, _ |- _ ]
                  => repeat match goal with
@@ -201,7 +189,7 @@ Section grammar_fixedpoint.
                       clear H
                | [ H : forall a b, is_true (is_valid_nonterminal ?ls ?nt) -> _ |- _ ]
                  => destruct (is_valid_nonterminal ls nt) eqn:?
-               | [ P_glb : forall a b, _ -> _ -> _ -> ?P ?nt (_ ⊓ _) |- ?P ?nt (_ ⊓ _) ] => apply P_glb
+               | [ P_lub : forall a b, _ -> _ -> _ -> ?P ?nt (_ ⊔ _) |- ?P ?nt (_ ⊔ _) ] => apply P_lu
                | [ H : context[match ?e with _ => _ end] |- _ ] => destruct e eqn:?
                | [ |- context[match ?e with _ => _ end] ] => destruct e eqn:?
                end. }
@@ -209,15 +197,15 @@ Section grammar_fixedpoint.
 
   Lemma pre_Fix_grammar_fixedpoint_correct_stronger
         (P : default_nonterminal_carrierT -> state gdata -> Type)
-        (Pinit : forall nt, is_true (is_valid_nonterminal initial_nonterminals_data nt)
-                            -> P nt (initial_state (*nt*)))
-        (Pbot : forall nt, is_valid_nonterminal initial_nonterminals_data nt = false
-                           -> P nt ⊥)
+        (Pbot : forall nt, is_true (is_valid_nonterminal initial_nonterminals_data nt)
+                            -> P nt ⊥)
+        (Ptop : forall nt, is_valid_nonterminal initial_nonterminals_data nt = false
+                           -> P nt ⊤)
         (IH : forall nt st,
-            (forall nt', is_valid_nonterminal initial_nonterminals_data nt' = false -> st nt' = ⊥)
+            (forall nt', is_valid_nonterminal initial_nonterminals_data nt' = false -> st nt' = ⊤)
             -> (forall nt', P nt' (st nt'))
             -> is_true (is_valid_nonterminal initial_nonterminals_data nt)
-            -> P nt (st nt ⊓ step_constraints gdata st nt (st nt)))
+            -> P nt (st nt ⊔ step_constraints gdata st nt (st nt)))
     : forall nt, P nt (lookup_state (pre_Fix_grammar gdata initial_nonterminals_data) nt).
   Proof.
     intro nt.
@@ -227,9 +215,9 @@ Section grammar_fixedpoint.
         move IH at bottom.
         specialize (IH nt'').
         let v := match type of IH with context[is_true ?v] => v end in
-        destruct v eqn:Hvalid'; eauto.
+        destruct v eqn:Hvalid'; eauto; [].
         { rewrite Hfalse by assumption.
-          rewrite bottom_glb_l.
+          rewrite top_lub_l.
           eauto. } } }
     { simpl rewrite lookup_state_invalid_pre_Fix_grammar; [ | assumption ]. eauto with nocore. }
   Qed.
